examples/lambda/completeness/unusedScript.sml
@@ -1,0 +1,250 @@
+(*---------------------------------------------------------------------------*
+ * boehm_treeScript.sml: (Effective) Boehm Trees (Chapter 10 of [1])         *
+ *---------------------------------------------------------------------------*)
+
+open HolKernel boolLib Parse bossLib;
+
+(* core theories *)
+open optionTheory arithmeticTheory pred_setTheory listTheory llistTheory
+     relationTheory ltreeTheory pathTheory posetTheory hurdUtils;
+
+open basic_swapTheory binderLib termTheory appFOLDLTheory chap2Theory
+     chap3Theory head_reductionTheory standardisationTheory solvableTheory;
+
+open pure_dBTheory;
+
+val _ = new_theory "unused";
+
+val _ = temp_delsimps ["lift_disj_eq", "lift_imp_disj"];
+val o_DEF = combinTheory.o_DEF; (* cannot directly open combinTheory *)
+
+(* A dB-term M is hnf if its corresponding Lambda term is hnf *)
+Overload dhnf = “\M. hnf (toTerm M)”
+
+Theorem dhnf_fromTerm[simp] :
+    !M. dhnf (fromTerm M) <=> hnf M
+Proof
+    rw [o_DEF]
+QED
+
+(* dB version of hnf_cases (only the ==> direction) *)
+Theorem dhnf_cases :
+    !M. dhnf M ==> ?n y Ms. M = dABSi n (dV y @* Ms)
+Proof
+    RW_TAC std_ss [hnf_cases]
+ >> qabbrev_tac ‘n = LENGTH vs’
+ >> Q.EXISTS_TAC ‘n’
+ >> Know ‘fromTerm (toTerm M) = fromTerm (LAMl vs (VAR y @* args))’
+ >- (art [fromTerm_11])
+ >> Q.PAT_X_ASSUM ‘toTerm M = LAMl vs (VAR y @* args)’ K_TAC
+ >> rw [fromTerm_LAMl, fromTerm_appstar]
+ >> qabbrev_tac ‘vs' = MAP s2n vs’
+ >> qabbrev_tac ‘Ms = MAP fromTerm args’
+ >> qabbrev_tac ‘y' = s2n y’
+ >> Know ‘dLAMl vs' (dV y' @* Ms) =
+          dABSi (LENGTH vs')
+            (FOLDL lift (dV y' @* Ms) (GENLIST I (LENGTH vs')) ISUB
+             ZIP (GENLIST dV (LENGTH vs'),
+                  MAP (\i. i + LENGTH vs') (REVERSE vs')))’
+ >- (MATCH_MP_TAC dLAMl_to_dABSi_applied \\
+     qunabbrev_tac ‘vs'’ \\
+     MATCH_MP_TAC ALL_DISTINCT_MAP_INJ >> rw [])
+ >> ‘LENGTH vs' = n’ by rw [Abbr ‘vs'’] >> POP_ORW
+ >> Rewr'
+ >> simp [FOLDL_lift_appstar, isub_appstar]
+ >> Know ‘FOLDL lift (dV y') (GENLIST I n) = dV (y' + n)’
+ >- (KILL_TAC \\
+     Induct_on ‘n’ >> rw [GENLIST, FOLDL_SNOC])
+ >> Rewr'
+ >> qabbrev_tac ‘Ms' = MAP (\e. FOLDL lift e (GENLIST I n)) Ms’
+ >> reverse (Cases_on ‘MEM y vs’)
+ >- (‘~MEM y' vs'’ by (rw [Abbr ‘y'’, Abbr ‘vs'’, MEM_MAP]) \\
+     ‘~MEM y' (REVERSE vs')’ by PROVE_TAC [MEM_REVERSE] \\
+     Suff ‘dV (y' + n) ISUB ZIP (GENLIST dV n,MAP (\i. i + n) (REVERSE vs')) =
+           dV (y' + n)’ >- (Rewr' >> METIS_TAC []) \\
+     MATCH_MP_TAC isub_dV_fresh \\
+     qabbrev_tac ‘l1 = GENLIST dV n’ \\
+     qabbrev_tac ‘l2 = MAP (\i. i + n) (REVERSE vs')’ \\
+    ‘LENGTH l1 = n’ by rw [Abbr ‘l1’] \\
+    ‘LENGTH l2 = n’ by rw [Abbr ‘l2’, Abbr ‘n’, Abbr ‘vs'’] \\
+     simp [DOM_ALT_MAP_SND, MAP_ZIP] \\
+     rw [Abbr ‘l2’, MEM_MAP])
+ (* stage work *)
+ >> ‘MEM y' vs'’ by (rw [Abbr ‘y'’, Abbr ‘vs'’, MEM_MAP])
+ >> ‘MEM y' (REVERSE vs')’ by PROVE_TAC [MEM_REVERSE]
+ >> ‘?j. j < LENGTH (REVERSE vs') /\ y' = EL j (REVERSE vs')’
+        by METIS_TAC [MEM_EL]
+ >> ‘LENGTH (REVERSE vs') = n’ by rw [Abbr ‘vs'’, Abbr ‘n’]
+ >> qabbrev_tac ‘Ns = MAP (\i. i + n) (REVERSE vs')’
+ >> ‘LENGTH Ns = n’ by rw [Abbr ‘Ns’]
+ >> Know ‘ALL_DISTINCT Ns’
+ >- (qunabbrev_tac ‘Ns’ \\
+     MATCH_MP_TAC ALL_DISTINCT_MAP_INJ >> rw [] \\
+     qunabbrev_tac ‘vs'’ \\
+     MATCH_MP_TAC ALL_DISTINCT_MAP_INJ >> rw [])
+ >> DISCH_TAC
+ >> Suff ‘dV (y' + n) ISUB ZIP (GENLIST dV n,Ns) = EL j (GENLIST dV n)’
+ >- (Rewr' \\
+     simp [EL_GENLIST] >> METIS_TAC [])
+ >> MATCH_MP_TAC isub_dV_once >> simp []
+ >> CONJ_TAC >- (rw [Abbr ‘Ns’, EL_MAP])
+ >> Q.X_GEN_TAC ‘i’ >> DISCH_TAC
+ >> ‘n <= EL i Ns’ by rw [Abbr ‘Ns’, EL_MAP]
+ >> Suff ‘FVS (ZIP (GENLIST dV n,Ns)) = count n’ >- rw []
+ >> Q.PAT_X_ASSUM ‘LENGTH Ns = n’ MP_TAC
+ >> KILL_TAC >> Q.ID_SPEC_TAC ‘Ns’
+ >> Induct_on ‘n’ >> rw [dFVS_def]
+ >> ‘Ns <> []’ by rw [NOT_NIL_EQ_LENGTH_NOT_0]
+ >> ‘LENGTH (FRONT Ns) = n’ by rw [LENGTH_FRONT]
+ >> ‘Ns = SNOC (LAST Ns) (FRONT Ns)’
+      by (rw [APPEND_FRONT_LAST, SNOC_APPEND]) >> POP_ORW
+ >> Q.PAT_X_ASSUM ‘!Ns. LENGTH Ns = n ==> P’ (MP_TAC o (Q.SPEC ‘FRONT Ns’))
+ >> rw [GENLIST, COUNT_SUC, dFVS_SNOC, ZIP_SNOC, dFV_def]
+ >> SET_TAC []
+QED
+
+(* |- ?f f' f''. !M. dhnf M ==> M = dABS (f M) (dV (f' M) @* f'' M) *)
+val dhnf_cases' = dhnf_cases
+               |> SIMP_RULE std_ss [GSYM RIGHT_EXISTS_IMP_THM, SKOLEM_THM];
+
+(* Explicit definitions of hnf components (easier to work with) by Michael Norrish:
+
+   1. The number of leading dABS (can be zero):
+ *)
+Definition dABSn_def :
+   (dABSn (dV n)       = 0) /\
+   (dABSn (dAPP t1 t2) = 0) /\
+   (dABSn (dABS t)     = 1 + dABSn t)
+End
+
+(* 2. The head variable of hnf (always exists) *)
+Definition dVn_def :
+   (dVn (dV n)       = n) /\
+   (dVn (dABS t)     = dVn t) /\
+   (dVn (dAPP t1 t2) = dVn t1)
+End
+
+(* 2. The list of terms after appstar (may be empty) *)
+Definition dAPPl_def :
+   (dAPPl (dV n)       = []) /\
+   (dAPPl (dABS t)     = dAPPl t) /\
+   (dAPPl (dAPP t1 t2) = SNOC t2 (dAPPl t1))
+End
+
+(* The "main" part of a hnf *)
+Definition dhnf_head_def :
+    dhnf_head M = dABSi (dABSn M) (dV (dVn M))
+End
+
+val _ = export_rewrites ["dABSn_def", "dVn_def", "dAPPl_def"];
+
+Theorem dABSn_dABSi[simp] :
+    dABSn (dABSi n t) = n + dABSn t
+Proof
+    Induct_on ‘n’ >> rw [FUNPOW_SUC]
+QED
+
+Theorem dABSn_dV_appstar[simp] :
+    dABSn (dV y @* Ns) = 0
+Proof
+    Induct_on ‘Ns’ using SNOC_INDUCT
+ >> rw [appstar_SNOC]
+QED
+
+Theorem dVn_dABSi[simp] :
+    dVn (dABSi n t) = dVn t
+Proof
+    Induct_on ‘n’ >> rw [FUNPOW_SUC]
+QED
+
+Theorem dVn_appstar[simp] :
+    dVn (M @* Ns) = dVn M
+Proof
+    Induct_on ‘Ns’ using SNOC_INDUCT >> rw []
+QED
+
+Theorem dAPPl_dABSi[simp] :
+    dAPPl (dABSi n t) = dAPPl t
+Proof
+    Induct_on ‘n’ >> rw [FUNPOW_SUC]
+QED
+
+Theorem dAPPl_dV_appstar[simp] :
+    dAPPl (dV y @* Ns) = Ns
+Proof
+    Induct_on ‘Ns’ using SNOC_INDUCT >> rw [dappstar_APPEND]
+QED
+
+Theorem dhnf_thm :
+    !M. dhnf M ==> M = dABSi (dABSn M) (dV (dVn M) @* dAPPl M)
+Proof
+    rpt STRIP_TAC
+ >> ‘?n y Ms. M = dABSi n (dV y @* Ms)’ by METIS_TAC [dhnf_cases]
+ >> rw []
+QED
+
+Definition principle_hnf_def :
+    principle_hnf = fromTerm o last o head_reduction_path o toTerm
+End
+
+Overload solvable = “solvable o toTerm”
+
+(* The needed unfolding function for ltree_unfold for Boehm Tree *)
+Definition dBT_generator_def :
+    dBT_generator (M :pdb) = if solvable M then
+                               let M' = principle_hnf M in
+                                 (SOME (dhnf_head M'), fromList (dAPPl M'))
+                             else
+                               (NONE, LNIL)
+End
+
+(* The Boehm tree of M, all in dB terms *)
+Definition dBT_def :
+    dBT = ltree_unfold dBT_generator
+End
+
+(* M = dABSi (dABSn M) (dV (dVn M) @* dAPPl M)
+   N = dABSi (dABSn N) (dV (dVn N) @* dAPPl N)
+
+   n  = dABSn M, y  = dVn M, m  = LENGTH (dAPPL M)
+   n' = dABSn N, y' = dVn N, m' = LENGTH (dAPPL N)
+ *)
+Definition dB_equivalent_def :
+    dB_equivalent (M :pdb) (N :pdb) =
+       if solvable M /\ solvable N then
+          let M0 = principle_hnf M;
+              N0 = principle_hnf N;
+              y  = dVn M0;
+              y' = dVn N0;
+              n  = dABSn M0;
+              n' = dABSn N0;
+              m  = LENGTH (dAPPl M0);
+              m' = LENGTH (dAPPl N0);
+          in
+              y = y' /\ n + m' = n' + m
+       else
+          ~solvable M /\ ~solvable N
+End
+
+Overload equivalent = “dB_equivalent”
+
+Theorem equivalent_alt_solvable :
+    !M N. solvable M /\ solvable N ==>
+         (equivalent M (N :pdb) <=>
+          let M0 = principle_hnf M;
+              N0 = principle_hnf N
+          in
+              dVn M0 = dVn N0 /\
+              dABSn M0 + LENGTH (dAPPl N0) = dABSn N0 + LENGTH (dAPPl M0))
+Proof
+    rw [dB_equivalent_def]
+QED
+
+val _ = export_theory ();
+val _ = html_theory "unused";
+
+(* References:
+
+   [1] Barendregt, H.P.: The lambda calculus, its syntax and semantics.
+       College Publications, London (1984).
+ *)
